wip

src/examples/Kuiper.Array.VectorizedAccess.fst
@@ -7,7 +7,7 @@ open FStar.Seq.Base
 
 module SZ = Kuiper.SizeT
 module V = Pulse.Lib.Vec
-
+module T = FStar.Tactics.V2
 open Kuiper.Array.Vectorized
 
 noextract
@@ -25,13 +25,17 @@ let kpre
   (bid : natlt nblk)
   (tid : natlt nthr)
   : slprop =
-  gpu_pts_to_slice a (global_id bid tid * 4) (global_id bid tid * 4 + 4)
+  gpu_pts_to_slice a 
+      (global_id bid tid * 4) (global_id bid tid * 4 + 4)
       (slice s (global_id bid tid * 4) (global_id bid tid * 4 + 4)) **
-  pure (aligned 16 a)
+  pure (aligned 16 a /\ is_global_array a)
+
+let scale_fun (v:float) (s:seq float) (i:nat{ i < length s }) : float =
+  v `mul` (s @! i)
 
 noextract
 let scale_seq (v : float) (s : seq float)
-  = Seq.init (length s) (fun i -> v `mul` Seq.index s i)
+  = Seq.init (length s) (fun i -> v `mul` (s @! i))
 
 noextract
 unfold
@@ -46,7 +50,83 @@ let kpost
   (tid : natlt nthr)
   : slprop =
   gpu_pts_to_slice a (global_id bid tid * 4) (global_id bid tid * 4 + 4)
-      (scale_seq v <| slice s (global_id bid tid * 4) (global_id bid tid * 4 + 4))
+      (scale_seq v (slice s (global_id bid tid * 4) (global_id bid tid * 4 + 4)))
+
+module T = FStar.Tactics
+let is_gpu_loc (#[T.exact (`0)]gpu_id) (l:loc_id) = gpu_of l == gpu_id_loc gpu_id
+
+open Kuiper.Seq.Common { seq_blit }
+atomic
+fn gpu_array_vec_cpy_dh_mine
+  (#et : Type u#0) {| sized et, has_vec_cpy et |}
+  (dst_arr : array et)
+  (dst_off : SZ.t)
+  (#src_sz : erased nat)
+  (src_arr : gpu_array et src_sz)
+  (src_off : SZ.t)
+  (#src_slice_i : erased nat)
+  (#src_slice_j : erased nat)
+  (#f : perm)
+  (#ss : erased (seq et))
+  (#ds : erased (seq et))
+  (#_ : squash (dst_off + chunk et <= Seq.length ds))
+  (#_ : squash (src_slice_i <= src_off /\ src_off + chunk et <= src_slice_j))
+  (#_ : squash (Seq.length ss == src_slice_j - src_slice_i))
+  preserves gpu
+  preserves gpu_pts_to_slice src_arr #f src_slice_i src_slice_j ss
+  requires  pure (aligned' 16 src_arr src_off)
+  requires  dst_arr |-> ds
+  ensures   exists* s. dst_arr |-> s ** pure (s == seq_blit ds dst_off ss (src_off - src_slice_i) (chunk et))
+{ gpu_array_vec_cpy_dh #et dst_arr dst_off #src_sz src_arr src_off #src_slice_i #src_slice_j #f #ss #ds; }
+
+atomic
+fn gpu_array_vec_cpy_hd_mine
+  (#et : Type u#0) {| sized et, has_vec_cpy et |}
+  (#dst_sz : erased nat)
+  (dst_arr : gpu_array et dst_sz)
+  (dst_off : SZ.t)
+  (#dst_slice_i : erased nat)
+  (#dst_slice_j : erased nat)
+  (src_arr : array et)
+  (src_off : SZ.t)
+  (#f : perm)
+  (#ss : erased (seq et))
+  (#ds : erased (seq et))
+  (#_ : squash (dst_slice_i <= dst_off /\ dst_off + chunk et <= dst_slice_j))
+  (#_ : squash (Seq.length ds == dst_slice_j - dst_slice_i))
+  (#_ : squash (src_off + chunk et <= Seq.length ss))
+  preserves gpu
+  preserves src_arr |-> Frac f ss
+  requires  pure (aligned' 16 dst_arr dst_off)
+  requires  gpu_pts_to_slice dst_arr dst_slice_i dst_slice_j ds
+  ensures   exists* s'. gpu_pts_to_slice dst_arr dst_slice_i dst_slice_j s' ** pure (s' == seq_blit ds (dst_off - dst_slice_i) ss src_off (chunk et))
+{
+  admit()
+}
+
+inline_for_extraction
+fn op_Array_Access
+        u#a (#t: Type u#a)
+        (a: array t)
+        (i: SZ.t)
+        (#p: perm)
+        (#s: Ghost.erased (Seq.seq t){SZ.v i < Seq.length s})
+  requires pts_to a #p s
+  returns  res : t
+  ensures  pts_to a #p s **
+           rewrites_to res (Seq.index s (SZ.v i))
+{ admit() }
+
+inline_for_extraction
+fn op_Array_Assignment
+        u#a (#t: Type u#a)
+        (a: array t)
+        (i: SZ.t)
+        (v: t)
+        (#s: Ghost.erased (Seq.seq t) {SZ.v i < Seq.length s})
+  requires pts_to a s
+  ensures  exists* s'. pts_to a s' ** pure (s' == Seq.upd s (SZ.v i) v)
+{ admit() }
 
 inline_for_extraction noextract
 fn kf
@@ -66,15 +146,15 @@ ensures
   gpu **
   kpost v size a s nblk nthr bid tid
 {
-  open Pulse.Lib.Array;
+//  open Pulse.Lib.Array;
+  // elim_on_gpu_array a;
   let global_idx = ((bid *^ nthr +^ tid) *^ 4sz); rewrite each ((SZ.v bid * SZ.v nthr + SZ.v tid) * 4) as SZ.v global_idx;
-
   with s0. assert (gpu_pts_to_slice a (SZ.v global_idx) (SZ.v global_idx + 4) s0);
 
   let mut local = [| zero #float #_; 4sz |];
 
-  gpu_array_vec_cpy_dh local 0sz a global_idx;
-
+  gpu_array_vec_cpy_dh_mine local 0sz a global_idx;
+  
   with s1. assert (local |-> s1);
   assert (pure (Seq.equal #float s0 s1));
 
@@ -86,15 +166,24 @@ ensures
   with s2. assert (local |-> s2);
   assert (pure (Seq.equal #float s2 (scale_seq v s1)));
 
-  gpu_array_vec_cpy_hd a global_idx local 0sz;
+  gpu_array_vec_cpy_hd_mine a global_idx local 0sz;
 
   with s3.
     assert (gpu_pts_to_slice a (SZ.v global_idx) (SZ.v global_idx + 4) s3);
   assert (pure (Seq.equal s3 s2));
   assert (pure (Seq.equal s3 (scale_seq v s0)));
-
   rewrite each SZ.v global_idx as ((SZ.v bid * SZ.v nthr + SZ.v tid) * 4);
-  ()
+}
+
+ghost
+fn fuse_on_placeless (q:slprop) {| placeless q |} #l #p ()
+requires on l p
+requires q
+ensures on l (p ** q)
+{ 
+  placeless_on_intro q l;
+  admit();
+  rewrite (on l p ** on l q) as on l (p ** q); 
 }
 
 fn hf (v : V.vec float)
@@ -109,13 +198,12 @@ fn hf (v : V.vec float)
 
   with s. assert v |-> s;
   assert (pure (Seq.equal s (slice s 0 4)));
-  assert a |-> slice s 0 4;
-
   let two = add #float one one;
+  fuse_on_placeless (pure (aligned 16 a /\ is_global_array a)) ();
+
   launch_kernel_1 (kf 4sz #(slice s 0 4) 1 a two 1sz 0sz 0sz);
 
   gpu_memcpy_device_to_host v a 4sz;
 
   gpu_array_free a;
-  ()
 }
