src/lib/kuiper/Kuiper.Array.Core.fst
@@ -42,23 +42,23 @@ returns x:a
 ensures post x
 { admit() }
 
-let gpu_array_core (a : Type u#0) (sz : nat) : Type u#0 = A.larray a sz
+let gpu_array (a : Type u#0) (sz : nat) : Type u#0 = A.larray a sz
 let loc_id_of_array #a #sz x = loc_id_of_array x
 let visibility_of #a #sz x = visibility_of_array x
 
 (* Base address of the GPU array, used to model alignment. This number
 is in units of *bytes*, not array elements. *)
-let base_address (#a : Type u#0) (#sz : nat) (x : gpu_array_core a sz)
+let base_address (#a : Type u#0) (#sz : nat) (x : gpu_array a sz)
 : GTot nat
 = core_base_address x
 
 let mask_of (i j:nat) (n:nat) : prop = i <= n /\ n < j
 
 (* x is the base pointer, this gives permission in [i,j) *)
-let gpu_pts_to_slice_core 
+let gpu_pts_to_slice
   (#a:Type u#0)
   (#sz:nat)
-  ([@@@mkey] x:gpu_array_core a sz)
+  ([@@@mkey] x:gpu_array a sz)
   (#[exact (`1.0R)] f : perm)
   ([@@@mkey] i : nat)
   (j : nat)
@@ -72,72 +72,61 @@ let gpu_pts_to_slice_core
           Seq.length s == sz /\
           A.is_full_array x)
 
-instance is_send_gpu_pts_to_slice_core 
+instance is_send_gpu_pts_to_slice
   (#a:Type u#0)
   (#sz:nat)
-  ([@@@mkey] x:gpu_array_core a sz)
+  ([@@@mkey] x:gpu_array a sz)
   (#[exact (`1.0R)] f : perm)
   ([@@@mkey] i : nat)
   (j : nat)
   (v : seq a)
 : is_send_across
-     (visibility_of_array x)
-     (gpu_pts_to_slice_core #a #sz x #f i j v)
+     (visibility_of x)
+     (gpu_pts_to_slice #a #sz x #f i j v)
 = solve
-
-let gpu_pts_to_slice
-  (#a:Type u#0)
-  (#sz:nat)
-  ([@@@mkey] x:gpu_array_core a sz)
-  (#[exact (`1.0R)] f : perm)
-  ([@@@mkey] i : nat)
-  (j : nat)
-  (v : seq a)
-: slprop
-= on (loc_id_of_array x) (gpu_pts_to_slice_core x #f i j v)
-
-let placeless_gpu_pts_to_slice
-  (#a:Type u#0)
-  (#sz:nat)
-  (x:gpu_array_core a sz)
-  (#[exact (`1.0R)] f : perm)
-  (i : nat)
-  (j : nat)
-  (v : seq a)
- : placeless (gpu_pts_to_slice x #f i j v)
- = solve
 
 ghost
 fn gpu_pts_to_slice_ref
   (#a:Type u#0)
   (#sz:nat)
   (#f : perm)
-  (x:gpu_array_core a sz)
+  (x:gpu_array a sz)
   (i:nat) (j:nat)
   (#v : seq a)
   preserves gpu_pts_to_slice x #f i j v
   requires emp
   ensures  pure (i <= j /\ j <= sz /\ Seq.length v == (j-i) /\ SZ.fits sz)
 {
-  ghost
-  fn aux ()
-  requires (loc (loc_id_of_array x) ** gpu_pts_to_slice x #f i j v)
-  ensures  (loc (loc_id_of_array x) ** 
-    (gpu_pts_to_slice x #f i j v **
-     pure (i <= j /\ j <= sz /\ Seq.length v == (j-i) /\ SZ.fits sz)))
-  { 
-    unfold gpu_pts_to_slice;
-    on_elim _;
-    unfold gpu_pts_to_slice_core;
-    fold (gpu_pts_to_slice_core x #f i j v);
-    on_intro #_ (gpu_pts_to_slice_core x #f i j v);
-    fold gpu_pts_to_slice;
-  };
-  ghost_impersonate _ _ _ aux
+  unfold gpu_pts_to_slice;
+  fold (gpu_pts_to_slice x #f i j v);
+}
+
+
+ghost
+fn gpu_pts_to_slice_ref_anywhere
+  (#a:Type u#0)
+  (#sz:nat)
+  (#f : perm)
+  (x:gpu_array a sz)
+  (i:nat) (j:nat)
+  (#v : seq a)
+  (#l:loc_id)
+  preserves on l (gpu_pts_to_slice x #f i j v)
+  requires emp
+  ensures  pure (i <= j /\ j <= sz /\ Seq.length v == (j-i) /\ SZ.fits sz)
+{
+  ghost_impersonate l
+     (on l (gpu_pts_to_slice x #f i j v))
+     (on l (gpu_pts_to_slice x #f i j v) **
+      pure (i <= j /\ j <= sz /\ Seq.length v == (j-i) /\ SZ.fits sz))
+    fn () {
+      on_elim _;
+      gpu_pts_to_slice_ref x i j;
+      on_intro (gpu_pts_to_slice x #f i j v);
+    }
 }
 
 let dummy = emp 
-
 
 noextract
 fn gpu_array_alloc_vis
@@ -147,9 +136,11 @@ fn gpu_array_alloc_vis
   (l:loc_id)
   (vis:visibility)
   preserves cpu
-  returns   x : gpu_array_core a (SZ.v sz)
+  returns  x : gpu_array a (SZ.v sz)
   ensures
-    exists* (s:seq a). x |-> s ** pure (Seq.length s == sz)
+    exists* (s:seq a). 
+      on l (x |-> s) **
+      pure (Seq.length s == sz)
   ensures
     pure (
       aligned 128 x /\
@@ -159,10 +150,10 @@ fn gpu_array_alloc_vis
 {
   fn aux ()
   requires loc l ** dummy
-  returns  x : gpu_array_core a (SZ.v sz)
+  returns  x : gpu_array a (SZ.v sz)
   ensures loc l
   ensures exists* (s:seq a). 
-    gpu_pts_to_array x s **
+    on l (gpu_pts_to_array x s) **
     pure (Seq.length s == sz /\
           visibility_of_array x == vis /\
           loc_id_of_array x == l)
@@ -171,10 +162,9 @@ fn gpu_array_alloc_vis
     let default_value : a = sized_types_inhabited;
     let x = alloc_array_with_vis default_value sz l vis;
     A.mask_mext x (mask_of 0 (SZ.v sz));
-    fold (gpu_pts_to_slice_core #a #(SZ.v sz) x 0 (SZ.v sz) (Seq.create (SZ.v sz) default_value));
-    on_intro #l (gpu_pts_to_slice_core _ _ _ _);
-    fold (gpu_pts_to_slice _ _ _ _);
+    fold (gpu_pts_to_slice #a #(SZ.v sz) x 0 (SZ.v sz) (Seq.create (SZ.v sz) default_value));
     fold (gpu_pts_to_array _ _);
+    on_intro #l (gpu_pts_to_array _ _);
     x
   };
   fold dummy;
@@ -190,11 +180,15 @@ fn gpu_array_alloc
   preserves cpu
   returns   x : gpu_array a (SZ.v sz)
   ensures
-    exists* (s:seq a). x |-> s ** pure (Seq.length s == sz)
-  ensures
-    pure (aligned 128 x)
+    exists* (s:seq a). 
+      on gpu_loc (x |-> s) **
+      pure (
+        Seq.length s == sz /\
+        aligned 128 x /\
+        is_global_array x
+      )
 {
-  let x = gpu_array_alloc_vis #a sz (gpu_of (gpu_id_loc 0)) (gpu_of);
+  let x = gpu_array_alloc_vis #a sz gpu_loc (gpu_of);
   gpu_of_idem (gpu_id_loc 0);
   x
 }
@@ -202,132 +196,28 @@ fn gpu_array_alloc
 fn gpu_array_free
   (#a:Type u#0)
   (#sz:erased nat)
-  (r : gpu_array_core a sz)
+  (r : gpu_array a sz)
   (#v : erased (seq a))
   preserves cpu
-  requires r |-> v
+  requires on gpu_loc (r |-> v)
   ensures  emp
 {
   fn aux ()
-  requires loc (loc_id_of_array r)
-  requires r |-> v
-  ensures  loc (loc_id_of_array r)
+  requires loc gpu_loc
+  requires on gpu_loc (r |-> v)
+  ensures  loc gpu_loc
   ensures dummy
   {
+    on_elim _;
     unfold gpu_pts_to_array;
     unfold gpu_pts_to_slice;
-    on_elim _;
-    unfold gpu_pts_to_slice_core;
     A.mask_mext r (fun _ -> True);
     A.mask_free r;
     fold dummy;
   };
-  __primitive__exec_on_gpu_loc (fun _ -> solve) (loc_id_of_array r) aux;
+  __primitive__exec_on_gpu_loc (fun _ -> solve) gpu_loc aux;
   unfold dummy;
 }
-
-[@@noextract_to "krml"]
-fn gpu_array_read_local
-  (#a : Type u#0)
-  (#sz : erased nat)
-  (#i  : erased nat)
-  (#j  : erased nat)
-  (r : gpu_array_core a sz)
-  (#f : perm)
-  (idx : SZ.t)
-  (#s : erased (seq a))
-  preserves gpu_pts_to_slice_core #a #sz r #f i j s
-  requires pure (i <= SZ.v idx /\ SZ.v idx < j)
-  returns  x:a
-  ensures  pure (i <= j /\ j <= sz /\ Seq.length s == (j-i) /\
-                 i <= SZ.v idx /\ SZ.v idx < j /\
-                 x == Seq.index s (SZ.v idx - i))
-{
-  unfold gpu_pts_to_slice_core;
-  let v = A.mask_read r idx;
-  fold gpu_pts_to_slice_core #a #sz r #f i j s;
-  v
-}
-
-[@@noextract_to "krml"]
-fn gpu_array_write_local
-  (#a:Type u#0)
-  (#sz: erased nat)
-  (#i: erased nat)
-  (#j: erased nat)
-  (r:gpu_array_core a sz)
-  (idx : SZ.t)
-  (v : a)
-  (#s : erased (seq a))
-  requires pure (i <= SZ.v idx /\ SZ.v idx < j)
-  requires gpu_pts_to_slice_core #a #sz r #1.0R i j s
-  ensures
-    with_pure
-      (i <= j /\ j <= sz /\ Seq.length s == (j-i) /\ i <= SZ.v idx /\ SZ.v idx < j)
-      (fun _ -> gpu_pts_to_slice_core #a #sz r #1.0R i j (Seq.upd s (SZ.v idx - i) v))
-{
-  unfold gpu_pts_to_slice_core;
-  A.mask_write r idx v;
-  fold (gpu_pts_to_slice_core #a #sz r #1.0R i j (Seq.upd s (SZ.v idx - i) v));
-}
-
-[@@noextract_to "krml"]
-fn gpu_array_read_loc
-  (#a : Type u#0)
-  (#sz : erased nat)
-  (#i  : erased nat)
-  (#j  : erased nat)
-  (r : gpu_array_core a sz)
-  (#f : perm)
-  (idx : SZ.t)
-  (#s : erased (seq a))
-  (#l : loc_id)
-  preserves loc l
-  preserves gpu_pts_to_slice #a #sz r #f i j s
-  requires pure (i <= SZ.v idx /\ SZ.v idx < j /\ r `visible_at` l)
-  returns  x:a
-  ensures  pure (i <= j /\ j <= sz /\ Seq.length s == (j-i) /\
-                 i <= SZ.v idx /\ SZ.v idx < j /\
-                 x == Seq.index s (SZ.v idx - i))
-{
-  unfold gpu_pts_to_slice;
-  SendSync.is_send_across_elim (visibility_of_array r) (gpu_pts_to_slice_core r #f i j s) l;
-  on_elim _;
-  let v = gpu_array_read_local r idx;
-  on_intro #l (gpu_pts_to_slice_core #a #sz r #f i j s);
-  SendSync.is_send_across_elim (visibility_of_array r) (gpu_pts_to_slice_core r #f i j s) (loc_id_of_array r);
-  fold gpu_pts_to_slice;
-  v
-}
-
-[@@noextract_to "krml"]
-fn gpu_array_write_loc
-  (#a:Type u#0)
-  (#sz: erased nat)
-  (#i: erased nat)
-  (#j: erased nat)
-  (r:gpu_array_core a sz)
-  (idx : SZ.t)
-  (v : a)
-  (#s : erased (seq a))
-  (#l : loc_id)
-  preserves loc l
-  requires pure (i <= SZ.v idx /\ SZ.v idx < j /\ r `visible_at` l)
-  requires gpu_pts_to_slice #a #sz r #1.0R i j s
-  ensures
-    with_pure
-      (i <= j /\ j <= sz /\ Seq.length s == (j-i) /\ i <= SZ.v idx /\ SZ.v idx < j)
-      (fun _ -> gpu_pts_to_slice #a #sz r #1.0R i j (Seq.upd s (SZ.v idx - i) v))
-{
-  unfold gpu_pts_to_slice;
-  SendSync.is_send_across_elim (visibility_of_array r) (gpu_pts_to_slice_core r i j s) l;
-  on_elim _;
-  gpu_array_write_local r idx v;
-  on_intro #l (gpu_pts_to_slice_core #a #sz r i j _);
-  SendSync.is_send_across_elim (visibility_of_array r) (gpu_pts_to_slice_core r i j (Seq.upd s (SZ.v idx - i) v)) (loc_id_of_array r);
-  fold gpu_pts_to_slice;
-}
-
 
 [@@noextract_to "krml"]
 fn gpu_array_read
@@ -335,12 +225,10 @@ fn gpu_array_read
   (#sz : erased nat)
   (#i  : erased nat)
   (#j  : erased nat)
-  (#gpu_id : erased int)
-  (r : gpu_array #gpu_id a sz)
+  (r : gpu_array a sz)
   (#f : perm)
   (idx : SZ.t)
   (#s : erased (seq a))
-  preserves gpu #gpu_id
   preserves gpu_pts_to_slice #a #sz r #f i j s
   requires pure (i <= SZ.v idx /\ SZ.v idx < j)
   returns  x:a
@@ -348,10 +236,10 @@ fn gpu_array_read
                  i <= SZ.v idx /\ SZ.v idx < j /\
                  x == Seq.index s (SZ.v idx - i))
 {
-  unfold (gpu #gpu_id); 
-  let x = gpu_array_read_loc r idx;
-  fold (gpu #gpu_id);
-  x
+  unfold gpu_pts_to_slice;
+  let v = A.mask_read r idx;
+  fold gpu_pts_to_slice #a #sz r #f i j s;
+  v
 }
 
 [@@noextract_to "krml"]
@@ -360,81 +248,29 @@ fn gpu_array_write
   (#sz: erased nat)
   (#i: erased nat)
   (#j: erased nat)
-  (#gpu_id : erased int)
-  (r:gpu_array #gpu_id a sz)
+  (r:gpu_array a sz)
   (idx : SZ.t)
   (v : a)
   (#s : erased (seq a))
-  preserves gpu #gpu_id
   requires pure (i <= SZ.v idx /\ SZ.v idx < j)
   requires gpu_pts_to_slice #a #sz r #1.0R i j s
   ensures
     with_pure
       (i <= j /\ j <= sz /\ Seq.length s == (j-i) /\ i <= SZ.v idx /\ SZ.v idx < j)
-      (fun _ -> gpu_pts_to_slice #a #sz r #1.0R i j (Seq.upd s (SZ.v idx - i) v))
+      (fun _ -> 
+        exists* s'. gpu_pts_to_slice #a #sz r #1.0R i j s' **
+            (pure (s' == Seq.upd s (SZ.v idx - i) v)))
 {
-  unfold (gpu #gpu_id);
-  gpu_array_write_loc r idx v;
-  fold (gpu #gpu_id);
-}
-
-
-[@@noextract_to "krml"]
-fn gpu_shmem_array_read
-  (#a : Type u#0)
-  (#sz : erased nat)
-  (#i  : erased nat)
-  (#j  : erased nat)
-  (#gpu_id #nblk #bid:erased int)
-  (r:gpu_shmem_array #gpu_id bid a sz)
-  (#f : perm)
-  (idx : SZ.t)
-  (#s : erased (seq a))
-  preserves block_id #gpu_id nblk bid
-  preserves gpu_pts_to_slice #a #sz r #f i j s
-  requires pure (i <= SZ.v idx /\ SZ.v idx < j)
-  returns  x:a
-  ensures  pure (i <= j /\ j <= sz /\ Seq.length s == (j-i) /\
-                 i <= SZ.v idx /\ SZ.v idx < j /\
-                 x == Seq.index s (SZ.v idx - i))
-{
-  unfold block_id #gpu_id nblk bid;
-  let v = gpu_array_read_loc r idx;
-  fold block_id #gpu_id nblk bid;
-  v
-}
-
-
-[@@noextract_to "krml"]
-fn gpu_shmem_array_write
-  (#a:Type u#0)
-  (#sz: erased nat)
-  (#i: erased nat)
-  (#j: erased nat)
-  (#gpu_id #nblk #bid:erased int)
-  (r:gpu_shmem_array #gpu_id bid a sz)
-  (idx : SZ.t)
-  (v : a)
-  (#s : erased (seq a))
-  preserves block_id #gpu_id nblk bid
-  requires pure (i <= SZ.v idx /\ SZ.v idx < j)
-  requires gpu_pts_to_slice #a #sz r #1.0R i j s
-  ensures
-    with_pure
-      (i <= j /\ j <= sz /\ Seq.length s == (j-i) /\ i <= SZ.v idx /\ SZ.v idx < j)
-      (fun _ -> gpu_pts_to_slice #a #sz r #1.0R i j (Seq.upd s (SZ.v idx - i) v))
-{
-  unfold block_id #gpu_id nblk bid;
-  gpu_array_write_loc r idx v;
-  fold block_id #gpu_id nblk bid;
+  unfold gpu_pts_to_slice;
+  A.mask_write r idx v;
+  fold (gpu_pts_to_slice #a #sz r #1.0R i j (Seq.upd s (SZ.v idx - i) v));
 }
 
 fn gpu_memcpy_host_to_device'
   (#a:Type u#0)
   {| sized a |}
   (#dst_sz : erased nat)
-  (#gpu_id: erased int)
-  (dst_garr : gpu_array #gpu_id a dst_sz)
+  (dst_garr : gpu_array a dst_sz)
   (dst_off : SZ.t)
   (#src_sz : erased nat)
   (src_arr : vec a)
@@ -451,18 +287,21 @@ fn gpu_memcpy_host_to_device'
     cpu **
     pts_to src_arr #f v
   requires
-    (dst_garr |-> gv)
+    on gpu_loc (dst_garr |-> gv)
   ensures
-    (dst_garr |-> seq_blit gv dst_off v src_off cnt) **
+    exists* s'. 
+      on gpu_loc (dst_garr |-> s') **
+      pure (s' == seq_blit gv dst_off v src_off cnt)
+  ensures
     pure (Seq.length v == reveal dst_sz)
 { admit () }
+
 
 fn gpu_memcpy_host_to_device
   (#a:Type u#0)
   {| sized a |}
   (#sz : erased nat)
-  (#gpu_id: erased int)
-  (dst_garr : gpu_array #gpu_id a sz)
+  (dst_garr : gpu_array a sz)
   (src_arr : vec a)
   (cnt : SZ.t)
   (#f : perm)
@@ -472,16 +311,21 @@ fn gpu_memcpy_host_to_device
     cpu **
     (src_arr |-> Frac f v)
   requires
-    (dst_garr |-> gv) **
-    pure (SZ.v cnt == sz /\ (Pulse.Lib.Vec.length src_arr == sz \/ Seq.length v == reveal sz))
+    on gpu_loc (dst_garr |-> gv)
+  requires 
+    pure (SZ.v cnt == sz /\
+          (Pulse.Lib.Vec.length src_arr == sz \/ Seq.length v == reveal sz))
   ensures
-    (dst_garr |-> v) **
+    on gpu_loc (dst_garr |-> v) **
     pure (Seq.length v == reveal sz)
 {
   Pulse.Lib.Vec.pts_to_len src_arr;
-  gpu_pts_to_slice_ref dst_garr _ _;
+  gpu_pts_to_slice_ref_anywhere dst_garr _ _;
   gpu_memcpy_host_to_device' dst_garr 0sz #sz src_arr 0sz cnt;
   assert pure (Seq.equal v (seq_blit gv 0sz v 0sz cnt));
+  with ss. 
+    rewrite (on gpu_loc (dst_garr |-> ss))
+    as      (on gpu_loc (dst_garr |-> v));
 }
 
 (* blit *)
@@ -492,8 +336,7 @@ fn gpu_memcpy_device_to_host'
   (dst_arr : vec a)
   (dst_off : SZ.t)
   (#src_sz : erased nat)
-  (#gpu_id : erased int)
-  (src_garr : gpu_array #gpu_id a src_sz)
+  (src_garr : gpu_array a src_sz)
   (src_off : SZ.t)
   (cnt : SZ.t {
     dst_off + cnt <= dst_sz /\
@@ -504,73 +347,73 @@ fn gpu_memcpy_device_to_host'
   (#gv : erased (seq a){ Seq.length gv == dst_sz })
   preserves
     cpu **
-    pts_to src_garr #f v
+    on gpu_loc (src_garr |-> Frac f (v<:seq _))
   requires
     (dst_arr |-> gv)
   ensures
-    (dst_arr |-> seq_blit gv dst_off v src_off cnt) **
-    pure (Seq.length v == reveal dst_sz)
-{
-  admit()
-}
+    exists* s'. dst_arr |-> s' **
+    pure (s'==seq_blit gv dst_off v src_off cnt /\ Seq.length v == reveal dst_sz)
+{ admit() } 
 
 fn gpu_memcpy_device_to_host
   (#a:Type u#0)
   {| sized a |}
   (#sz : erased nat)
-  (#gpu_id : erased int)
   (dst_arr : vec a)
-  (src_garr : gpu_array #gpu_id a sz)
+  (src_garr : gpu_array a sz)
   (cnt : SZ.t)
   (#f : perm)
   (#v : erased (seq a))
   (#gv : erased (seq a))
   preserves
     cpu **
-    (src_garr |-> Frac f gv)
+    on gpu_loc (src_garr |-> Frac f gv)
   requires
     (dst_arr |-> v) **
-    pure (SZ.v cnt == sz /\ (Pulse.Lib.Vec.length dst_arr == sz \/ Seq.length v == reveal sz))
+    pure (
+      SZ.v cnt == sz /\
+      (Pulse.Lib.Vec.length dst_arr == sz \/ Seq.length v == reveal sz))
   ensures
     (dst_arr |-> gv) **
     pure (Seq.length gv == reveal sz)
 {
   Pulse.Lib.Vec.pts_to_len dst_arr;
-  gpu_pts_to_slice_ref src_garr _ _;
+  gpu_pts_to_slice_ref_anywhere src_garr _ _;
   gpu_memcpy_device_to_host' #_ #_ #sz dst_arr 0sz #sz src_garr 0sz cnt;
   assert pure (Seq.equal gv (seq_blit v 0sz gv 0sz cnt));
 }
+
 
 fn gpu_memcpy_device_to_device
   (#a:Type u#0)
   {| sized a |}
   (#sz : erased nat)
-  (#gpu1 #gpu2:erased int)
-  (dst_arr : gpu_array #gpu1 a sz)
-  (src_garr : gpu_array #gpu2 a sz)
+  (dst_arr : gpu_array a sz)
+  (src_garr : gpu_array a sz)
   (cnt : SZ.t)
   (#f : perm)
   (#v : erased (seq a))
   (#gv : erased (seq a))
   preserves
     cpu **
-    (src_garr |-> Frac f gv)
+    on gpu_loc (src_garr |-> Frac f gv)
   requires
-    (dst_arr |-> v) **
-    pure (SZ.v cnt == sz /\ (Seq.length gv == sz \/ Seq.length v == sz))
+    on gpu_loc (dst_arr |-> v) **
+    pure (
+      SZ.v cnt == sz /\ 
+      (Seq.length gv == sz \/ Seq.length v == sz))
   ensures
-    (dst_arr |-> gv) **
+    on gpu_loc (dst_arr |-> gv) **
     pure (Seq.length gv == reveal sz)
 {
   admit()
 }
 
-
 ghost
 fn gpu_array_slice_1
   (#a:Type u#0)
   (#sz:nat)
-  (arr : gpu_array_core a sz)
+  (arr : gpu_array a sz)
   (#f : perm)
   (#v : erased (seq a) { Seq.length v == sz })
   requires pts_to arr #f v
@@ -583,7 +426,7 @@ ghost
 fn gpu_array_unslice_1
   (#a:Type u#0)
   (#sz:nat)
-  (arr : gpu_array_core a sz)
+  (arr : gpu_array a sz)
   (#f : perm)
   (#v : erased (seq a) { Seq.length v == sz })
   requires forall+ (i: natlt sz). gpu_pts_to_cell arr #f i (v @! i)
@@ -597,7 +440,7 @@ ghost
 fn gpu_slice_concat
   (#a:Type u#0)
   (#sz:nat)
-  (arr : gpu_array_core a sz)
+  (arr : gpu_array a sz)
   (#[exact (`1.0R)] f : perm)
   (#s1 #s2: erased (seq a))
   (i n m:nat)
@@ -611,7 +454,7 @@ ghost
 fn gpu_slice_split
   (#a:Type u#0)
   (#sz:nat)
-  (arr : gpu_array_core a sz)
+  (arr : gpu_array a sz)
   (#[exact (`1.0R)] f : perm)
   (#s1 #s2: erased (seq a))
   (i n m:nat)
@@ -624,7 +467,7 @@ fn gpu_slice_split
 ghost
 fn gpu_slice_empty_elim
   (#a:Type u#0) (#sz:nat)
-  (arr : gpu_array_core a sz)
+  (arr : gpu_array a sz)
   (i : nat)
   requires gpu_pts_to_slice arr #'f i i 'v
   ensures  emp
@@ -635,7 +478,7 @@ fn gpu_slice_empty_elim
 ghost
 fn gpu_slice_empty_intro
   (#a:Type u#0) (#sz:nat)
-  (arr : gpu_array_core a sz)
+  (arr : gpu_array a sz)
   (i : nat)
   requires emp
   ensures  gpu_pts_to_slice arr #'f i i seq![]
@@ -647,7 +490,7 @@ ghost
 fn gpu_slice_share
   (#a:Type u#0)
   (#sz:nat)
-  (arr : gpu_array_core a sz)
+  (arr : gpu_array a sz)
   (m n:nat)
   (k: nat { k > 0 })
   (#f : perm)
@@ -662,7 +505,7 @@ ghost
 fn gpu_slice_gather
   (#a:Type u#0)
   (#sz:nat)
-  (arr : gpu_array_core a sz)
+  (arr : gpu_array a sz)
   (m n:nat)
   (k: nat { k > 0 })
   (#f : perm) // FIXME: if we use 'f, it gets type 'real' instead of 'perm'
@@ -677,7 +520,7 @@ ghost
 fn gpu_slice_pts_to_eq
   (#a:Type u#0)
   (#sz:nat)
-  (arr : gpu_array_core a sz)
+  (arr : gpu_array a sz)
   (m n:nat)
   (#f1 f2 : perm)
   (#v1 #v2 : seq a)
@@ -694,21 +537,21 @@ fn gpu_slice_pts_to_eq
 // val adjacent
 //   (#a : Type u#0)
 //   (#s1 #s2 : nat)
-//   (arr1 : gpu_array_core a s1)
-//   (arr2 : gpu_array_core a s2)
+//   (arr1 : gpu_array a s1)
+//   (arr2 : gpu_array a s2)
 //   : slprop
 
 // ghost
 // fn gpu_array_cut
 //   (#a : Type u#0) {| sized a |}
 //   (#sz : nat)
-//   (arr : gpu_array_core a sz)
+//   (arr : gpu_array a sz)
 //   (k : SZ.t{ k <= sz })
 //   (#s : lseq a sz)
 //   requires
 //     (arr |-> Frac 'f s)
 //   returns
-//     p : (gpu_array_core a k & gpu_array_core a (sz - k))
+//     p : (gpu_array a k & gpu_array a (sz - k))
 //   ensures
 //     (p._1 |-> Frac 'f (seq_take k s)) **
 //     (p._2 |-> Frac 'f (seq_drop k s)) **
@@ -722,13 +565,13 @@ fn gpu_slice_pts_to_eq
 // fn gpu_array_paste
 //   (#a : Type u#0)
 //   (#sz1 #sz2 : nat)
-//   (arr1 : gpu_array_core a sz1)
-//   (arr2 : gpu_array_core a sz2)
+//   (arr1 : gpu_array a sz1)
+//   (arr2 : gpu_array a sz2)
 //   requires
 //     (arr1 |-> Frac 'f 's1) **
 //     (arr2 |-> Frac 'f 's2) **
 //     adjacent arr1 arr2
 //   returns
-//     arr : gpu_array_core a (sz1 + sz2)
+//     arr : gpu_array a (sz1 + sz2)
 //   ensures
 //     arr |-> Frac 'f ('s1 @+ 's2)
